Cslib/Computability/Machines/MultiTapeTuring/Routines/Typed.lean
@@ -14,53 +14,107 @@ namespace Routines
 
 /-- Turing machine `tm` computes a function on data from tape `i` and updates tape `j`. -/
 -- TODO move this somewhere else
-public def computes_function {k : ℕ}
-  (tm : MultiTapeTM k Char) (f : TapeView → Data → TapeView)
-  (i j : Fin k) (_h_neq : i ≠ j)
-  (views : Fin k → TapeView) :=
-  tm.eval_struct views = some (Function.update views j
-    (((views i).current.map (f (views j))).getD (views j)))
+public def computes_function_read_update {k : ℕ}
+  (tm : MultiTapeTM k Char) (f : Data → TapeView → TapeView)
+  (i j : Fin k) (_h_neq : i ≠ j) :=
+  ∀ views, tm.eval_struct views = some (Function.update views j
+    (((views i).current.map (f · (views j))).getD (views j)))
 
 -- TODO could generalize this to `f` having a preimage β.
-public def computes_function_push {k : ℕ}
+/-- Turing machine `tm` computes a function on data from tape `i` and pushes data to the
+list on tape `j`. -/
+public def computes_function_read_push {k : ℕ}
   {α : Type} [StrEnc α]
-  (tm : MultiTapeTM k Char) (f : Data → α)
+  (tm : MultiTapeTM k Char)
+  (f : Data → α)
   (i j : Fin k) (h_neq : i ≠ j) :=
-  computes_function tm (fun tv d => tv.pushList (StrEnc.toData (f d))) i j h_neq
+  computes_function_read_update tm (fun d tv => tv.pushList (StrEnc.toData (f d))) i j h_neq
 
-/-- Turing machine `tm` computes a function of the current item at tape `i` seen as type
--- `α` and pushes the result (type `β`) to tape `j`. -/
--- public def computes_function_push' {k : ℕ}
---   {α β : Type} [StrEnc α] [StrEnc β]
---   (tm : MultiTapeTM k Char) (f : α → β)
---   (i j : Fin k) (_h_neq : i ≠ j) :=
---   computes_function tm (fun tv d => tv.pushList (StrEnc.toData (f d))) i j _h_neq
-
-public def computes_function_push_bool {k : ℕ}
-  (tm : MultiTapeTM k Char) (f : Data → Bool)
+-- TODO maybe we don't need this any more if we generalize the input type, so if the
+-- input does not decode to a list, we do nothing.
+/-- Turing machine `tm` computes a function on a list from tape `i` and pushes data to the
+lsit on tape `j`. -/
+public def computes_function_readList_push {k : ℕ}
+  {α : Type} [StrEnc α]
+  (tm : MultiTapeTM k Char)
+  (f : List Data → α)
   (i j : Fin k) (h_neq : i ≠ j) :=
-  computes_function_push (α := Bool) tm f i j h_neq
+  computes_function_read_update tm (fun d tv => match d with
+   | Data.list ls => tv.pushList (StrEnc.toData (f ls))
+   | Data.num _ => tv) i j h_neq
+
 
 /-- Turing machine `tm` updates the head of tape `i`. -/
-public def computes_function_update {k : ℕ}
+public def computes_function_head_update {k : ℕ}
   {α β : Type} [StrEnc α] [StrEnc β]
   (tm : MultiTapeTM k Char) (f : α → β)
-  (i : Fin k)
-  (views : Fin k → TapeView) :=
-  tm.eval_struct views = some (Function.update views i ((views i).updateListHeadTyped f))
+  (i : Fin k) :=
+  ∀ views, tm.eval_struct views =
+    some (Function.update views i ((views i).updateListHeadTyped f))
 
 @[simp]
-public theorem computes_function_seq {k : ℕ}
+public theorem computes_function_seq₁ {k : ℕ}
   {β γ : Type} [StrEnc β] [StrEnc γ]
   (tm₁ tm₂ : MultiTapeTM k Char) (f₁ : Data → β) (f₂ : β → γ)
   (i j : Fin k) (h_neq : i ≠ j)
-  (h_comp₁ : ∀ views, computes_function_push tm₁ f₁ i j h_neq views)
-  (h_comp₂ : ∀ views, computes_function_update tm₂ f₂ i views)
-  (views : Fin k → TapeView) :
-  computes_function_push (tm₁ ;ₜ tm₂) (f₂ ∘ f₁) i j h_neq views := by sorry
+  (h_comp₁ : computes_function_read_push tm₁ f₁ i j h_neq)
+  (h_comp₂ : computes_function_head_update tm₂ f₂ i) :
+  computes_function_read_push (tm₁ ;ₜ tm₂) (f₂ ∘ f₁) i j h_neq := by sorry
 
--- We have a function that has j : +Bool
--- Do we model the effect on the tape?
+@[simp]
+public theorem computes_function_seq₂ {k : ℕ}
+  {β γ : Type} [StrEnc β] [StrEnc γ]
+  {tm₁ tm₂ : MultiTapeTM k Char} {f₁ : List Data → β} {f₂ : β → γ}
+  {i j : Fin k} (h_neq : i ≠ j)
+  (h_comp₁ : computes_function_readList_push tm₁ f₁ i j h_neq)
+  (h_comp₂ : computes_function_head_update tm₂ f₂ i) :
+  computes_function_readList_push (tm₁ ;ₜ tm₂) (f₂ ∘ f₁) i j h_neq := by sorry
+
+inductive TapeEffects where
+  | read
+  | consume
+  | put
+  | modify
+
+-- and all indices different
+def FunArgs (k : ℕ) := List ((Fin k) × TapeEffects)
+
+def ReturnType {k : ℕ} (args : FunArgs k) : Type := match args with
+ | [] => Unit
+ | (_, .read) :: rest => ReturnType rest
+ | (_, .consume) :: rest => ReturnType rest
+ | (_, .put) :: rest => Data × ReturnType rest
+ | (_, .modify) :: rest => Data × ReturnType rest
+
+def InputTypes {k : ℕ} (args : FunArgs k) : Type := match args with
+ | [] => Unit
+ | (_, .read) :: rest => Data → (InputTypes rest)
+ | (_, .consume) :: rest => Data → (InputTypes rest)
+ | (_, .put) :: rest => InputTypes rest
+ | (_, .modify) :: rest => Data → (InputTypes rest)
+
+def TypeOfFunArgs {k : ℕ} (args : FunArgs k) : Type := (InputTypes args) → (ReturnType args)
+
+-- def EvaluateFun {k : ℕ} (args : FunArgs k) (views : Fin k → TapeView)
+--   (f : TypeOfFunArgs args) : Option (ReturnType args) := match args with
+--   | [] => some ()
+--   | (i, .read) :: rest => (views i).current.bind (fun d => EvaluateFun rest views (f d))
+--   | (_, .consume) :: rest => Data → (InputTypes rest)
+--   | (_, .put) :: rest => InputTypes rest
+--   | (_, .modify) :: rest => Data → (InputTypes rest)
+
+--   --(i, TapeEffects.read) :: rest =>
+--     let current := (views i).current
+--     current.bind (fun d => EvaluateFun rest views (f d))
+
+-- public def computes_function_general {k : ℕ}
+--   (tm : MultiTapeTM k Char) (f : TapeView → Data → TapeView)
+--   (i j : Fin k) (_h_neq : i ≠ j)
+--   (views : Fin k → TapeView) :=
+--   tm.eval_struct views = some (Function.update views j
+--     (((views i).current.map (f (views j))).getD (views j)))
+
+
 
 end Routines
 end Turing
